making changes related to if-then-else

puar/Processor.v
@@ -741,61 +741,58 @@ Section Processor.
             );
           Retv }.
 
-  Notation Stale :=
-    STRUCT {
-        stalePc :: VAddr;
-        staleInstVToP :: optT (Struct VToPRp);
-        staleInst :: optT Inst;
-        staleMemVAddr :: optT VAddr;
-        staleMemVToP :: optT (Struct VToPRp) }.
+  Record VToPRpEntry {ty} := { pAddrEntry: ty PAddr ;
+                               modeEntry: ty Mode ;
+                               exceptEntry: option (ty MemException)
+                             }.
 
-  Notation StaleT := (Struct Stale).
+  Record Stale ty := { sPc: ty VAddr ;
+                       sInstVToP: option (@VToPRpEntry ty) ;
+                       sInst: option (ty Inst) ;
+                       sMemVAddr: option (ty VAddr) ;
+                       sMemVToP: option (@VToPRpEntry ty)
+                     }.
 
-  Notation Stales ty := (@NativeKind (list (ty StaleT)) nil).
+  Definition newStalePc {ty} (val: ty VAddr) := {| sPc := val;
+                                                   sInstVToP := None;
+                                                   sInst := None;
+                                                   sMemVAddr := None;
+                                                   sMemVToP := None |}.
+
+  Definition updInstVToP {ty} (s: Stale ty) val :=
+    {| sPc := sPc s;
+       sInstVToP := Some val;
+       sInst := sInst s;
+       sMemVAddr := sMemVAddr s;
+       sMemVToP := sMemVToP s |}.
+
+  Definition updInst {ty} (s: Stale ty) val :=
+    {| sPc := sPc s;
+       sInstVToP := sInstVToP s;
+       sInst := Some val;
+       sMemVAddr := sMemVAddr s;
+       sMemVToP := sMemVToP s |}.
+
+  Definition updMemVAddr {ty} (s: Stale ty) val :=
+    {| sPc := sPc s;
+       sInstVToP := sInstVToP s;
+       sInst := sInst s;
+       sMemVAddr := Some val;
+       sMemVToP := sMemVToP s |}.
+
+  Definition updMemVToP {ty} (s: Stale ty) val :=
+    {| sPc := sPc s;
+       sInstVToP := sInstVToP s;
+       sInst := sInst s;
+       sMemVAddr := sMemVAddr s;
+       sMemVToP := Some val |}.
+
+  Notation StaleT ty val := (@NativeKind (Stale ty) (newStalePc val)).
+  Notation StaleT' val := (StaleT _ val).
+  Notation Stales ty := (@NativeKind (list (Stale ty)) nil).
   Notation Stales' := (Stales _).
-  Notation addrs := (wordToNat (wones VAddrSz)).
 
-  Open Scope kami_expr.
-  Notation newStalePc val :=
-    STRUCT {
-        stalePc ::= val;
-        staleInstVToP ::= none;
-        staleInst ::= none;
-        staleMemVAddr ::= none;
-        staleMemVToP ::= none }.
-
-  Notation updInstVToP s val :=
-    STRUCT {
-        stalePc ::= s!Stale@.stalePc;
-        staleInstVToP ::= some val;
-        staleInst ::= s!Stale@.staleInst;
-        staleMemVAddr ::= s!Stale@.staleMemVAddr;
-        staleMemVToP ::= s!Stale@.staleMemVToP }.
-
-  Notation updInst s val :=
-    STRUCT {
-        stalePc ::= s!Stale@.stalePc;
-        staleInstVToP ::= s!Stale@.staleInstVToP;
-        staleInst ::= some val;
-        staleMemVAddr ::= s!Stale@.staleMemVAddr;
-        staleMemVToP ::= s!Stale@.staleMemVToP }.
-
-  Notation updMemVAddr s val :=
-    STRUCT {
-        stalePc ::= s!Stale@.stalePc;
-        staleInstVToP ::= s!Stale@.staleInstVToP;
-        staleInst ::= s!Stale@.staleInst;
-        staleMemVAddr ::= some val;
-        staleMemVToP ::= s!Stale@.staleMemVToP }.
-
-  Notation updMemVToP s val :=
-    STRUCT {
-        stalePc ::= s!Stale@.stalePc;
-        staleInstVToP ::= s!Stale@.staleInstVToP;
-        staleInst ::= s!Stale@.staleInst;
-        staleMemVAddr ::= s!Stale@.staleMemVAddr;
-        staleMemVToP ::= some val }.
-  Close Scope kami_expr.
+  Notation NativeVar ntype nval := (Var _ (@NativeKind ntype nval) nval).
 
   Definition processorSpec :=
     SIN {
@@ -807,107 +804,131 @@ Section Processor.
         with RegisterN stales : Stales type <- (NativeConst nil nil)
 
         with Rule stalePc :=
-          Nondet vAddr: SyntaxKind VAddr;
           ReadN stalesVal : Stales' <- stales;
-          LET newStale: StaleT <- newStalePc #vAddr;
-          WriteN stales : _ <- Var _ Stales' (stalesVal ++ [newStale]);
+          Nondet vAddr: SyntaxKind VAddr;
+          WriteN stales : _ <- Var _ Stales' (stalesVal ++ [newStalePc vAddr]);
           Retv
 
         with Rule staleInstVToP :=
-          Nondet i: @NativeKind nat 0;
           ReadN stalesVal : Stales' <- stales;
-          LET noEntry : StaleT <- $$ Default;
-          LET entry : StaleT <- #(nth i stalesVal noEntry);
-          LET stalePcVal : VAddr <- #entry!Stale@.stalePc;
+          Nondet i: @NativeKind nat 0;
           Assert $$ (indexIn i stalesVal);
-          Call inp <- instVToPCall(#stalePcVal);
-          LET newEntry: StaleT <- updInstVToP #entry #inp;
-          WriteN stales : _ <- Var _ Stales' (updList newEntry i stalesVal);
+          LET vAddrDef : VAddr <- $$ Default;
+          Call inp <- instVToPCall(#(sPc (nth i stalesVal (newStalePc vAddrDef))));
+          LET p <- #inp!VToPRp@.pAddr;
+          LET m <- #inp!VToPRp@.mode;
+          LET e <- getSome #inp!VToPRp@.exception;
+          LETN e': _ <- IF isSome #inp!VToPRp@.exception == $$ true
+                        then Var _ (@NativeKind (option (_ MemException)) None) (Some e)
+                        else Var _ (@NativeKind (option (_ MemException)) None) None;
+          WriteN stales : _ <- Var _ Stales' (nth_upd updInstVToP {| pAddrEntry := p;
+                                                                     modeEntry := m;
+                                                                     exceptEntry := e' |}
+                                                      i stalesVal);
           Retv
 
         with Rule staleInst :=
-          Nondet i: @NativeKind nat 0;
           ReadN stalesVal : Stales' <- stales;
-          LET noEntry : StaleT <- $$ Default;
-          LET entry : StaleT <- #(nth i stalesVal noEntry);
-          LET staleInstVToPVal : optT (Struct VToPRp) <- #entry!Stale@.staleInstVToP;
-          Assert (isSome #staleInstVToPVal);
-          Call inp <- instCall((getSome #staleInstVToPVal)!VToPRp@.pAddr);
-          LET newEntry: StaleT <- updInst #entry #inp;
-          WriteN stales : _ <- Var _ Stales' (updList newEntry i stalesVal);
+          Nondet i: @NativeKind nat 0;
+          Assert $$ (indexIn i stalesVal);
+          LET vAddrDef : VAddr <- $$ Default;
+          LET pAddrDef : PAddr <- $$ Default;
+          LET modeDef : Mode <- $$ Default;
+          LETN vToPRpDef : _ <- NativeVar VToPRpEntry {| pAddrEntry := pAddrDef;
+                                                         modeEntry := modeDef;
+                                                         exceptEntry := None |};
+          Call inp <- instCall(#(pAddrEntry
+                                   (rmSome
+                                      vToPRpDef
+                                      (sInstVToP
+                                         (nth i stalesVal (newStalePc vAddrDef))))));
+          WriteN stales : _ <- Var _ Stales' (nth_upd updInst inp i stalesVal);
           Retv
 
         with Rule staleMemVAddr :=
-          Nondet vAddr: SyntaxKind VAddr;
-          Nondet i: @NativeKind nat 0;
           ReadN stalesVal : Stales' <- stales;
-          LET noEntry : StaleT <- $$ Default;
-          LET entry : StaleT <- #(nth i stalesVal noEntry);
-          LET staleInstVal : optT Inst <- #entry!Stale@.staleInst;
-          Assert (isSome #staleInstVal);
-          LET newEntry: StaleT <- updMemVAddr #entry #vAddr;
-          WriteN stales : _ <- Var _ Stales' (updList newEntry i stalesVal);
+          Nondet i: @NativeKind nat 0;
+          Assert $$ (indexIn i stalesVal);
+          Nondet vAddr: SyntaxKind VAddr;
+          WriteN stales : _ <- Var _ Stales' (nth_upd updMemVAddr vAddr i stalesVal);
           Retv
 
         with Rule staleMemVToP :=
-          Nondet i: @NativeKind nat 0;
           ReadN stalesVal : Stales' <- stales;
-          LET noEntry : StaleT <- $$ Default;
-          LET entry : StaleT <- #(nth i stalesVal noEntry);
-          LET staleMemVAddr : optT VAddr <- #entry!Stale@.staleMemVAddr;
-          Assert (isSome #staleMemVAddr);
-          Call inp <- memVToPCall(getSome #staleMemVAddr);
-          LET newEntry: StaleT <- updMemVToP #entry #inp;
-          WriteN stales : _ <- Var _ Stales' (updList newEntry i stalesVal);
-          Retv
-
-        with Rule drop :=
           Nondet i: @NativeKind nat 0;
-          ReadN stalesVal : Stales' <- stales;
-          WriteN stales : _ <- Var _ Stales' (rmList i stalesVal);
-          LET noEntry : Struct Stale <- $$ Default;
-          LET entry : Struct Stale <- #(hd noEntry stalesVal);
+          Assert $$ (indexIn i stalesVal);
+          LET vAddrDef : VAddr <- $$ Default;
+          Call inp <- memVToPCall(#(sPc (nth i stalesVal (newStalePc vAddrDef))));
+          LET p <- #inp!VToPRp@.pAddr;
+          LET m <- #inp!VToPRp@.mode;
+          LET e <- getSome #inp!VToPRp@.exception;
+          LETN e': _ <- IF isSome #inp!VToPRp@.exception == $$ true
+                        then Var _ (@NativeKind (option (_ MemException)) None) (Some e)
+                        else Var _ (@NativeKind (option (_ MemException)) None) None;
+          WriteN stales : _ <- Var _ Stales' (nth_upd updMemVToP {| pAddrEntry := p;
+                                                                    modeEntry := m;
+                                                                    exceptEntry := e' |}
+                                                      i stalesVal);
           Retv
             
         with Rule memRq :=
           ReadN stalesVal : Stales' <- stales;
-          WriteN stales : _ <- Var _ Stales' (tl stalesVal);
-          LET noEntry : Struct Stale <- $$ Default;
-          LET inp1 : Struct Stale <- #(hd noEntry stalesVal);
-          LET instVal: Inst <- getSome #inp1!Stale@.staleInst;
+
           Read wbPcVal: VAddr <- wbPc;
           Read cStateVal: CState <- cState;
           Read regFileVals: Vector Data RIndexSz <- regFile;
           Read modeVal: Mode <- mode;
 
-          Assert $$ (notNil stalesVal);
-          Assert (isSome #inp1!Stale@.staleInstVToP);
-          Assert (isSome #inp1!Stale@.staleInst);
+          LET vAddrDef : VAddr <- $$ Default;
+          LETN inp1 : _ <- Var _ (StaleT' vAddrDef) (hd (newStalePc vAddrDef) stalesVal);
+          LET pAddrDef: PAddr <- $$ Default;
+          LET modeDef: Mode <- $$ Default;
+          LETN vToPRpDef: _ <- NativeVar VToPRpEntry {| pAddrEntry := pAddrDef;
+                                                        modeEntry := modeDef;
+                                                        exceptEntry := None |} ;
+          LET memExceptDef: MemException <- $$ Default ;
+          LET instDef: Inst <- $$ Default;
+
+          LET pcVal <- #(sPc inp1);
+          LET physicalPcVal <- #(pAddrEntry (rmSome vToPRpDef (sInstVToP inp1)));
+          LET instModeVal <- #(modeEntry (rmSome vToPRpDef (sInstVToP inp1)));
+          LET instExceptionVal <-
+              STRUCT {
+                valid ::= $$ (isValid (exceptEntry (rmSome vToPRpDef (sInstVToP inp1))));
+                data ::= #(rmSome memExceptDef
+                                  (exceptEntry (rmSome vToPRpDef (sInstVToP inp1)))) };
+          LET instVal <- #(rmSome instDef (sInst inp1));
+          LET memVAddrVal1 <- #(rmSome vAddrDef (sMemVAddr inp1));
+          LET memPAddrVal <- #(pAddrEntry (rmSome vToPRpDef (sMemVToP inp1)));
+          LET memModeVal <- #(modeEntry (rmSome vToPRpDef (sMemVToP inp1)));
+          LET memExceptionVal <-
+              STRUCT {
+                valid ::= $$ (isValid (exceptEntry (rmSome vToPRpDef (sMemVToP inp1))));
+                data ::= #(rmSome memExceptDef
+                                  (exceptEntry (rmSome vToPRpDef (sMemVToP inp1)))) };
 
           LET src1Val <- #regFileVals@[getSrc1 _ instVal];
           LET src2Val <- #regFileVals@[getSrc2 _ instVal];
 
           LET execVal <- execFn _ instVal src1Val src2Val;
 
-          If (isLdSt _ instVal)
-          then (
-            Assert (isSome #inp1!Stale@.staleMemVAddr);
-            Assert (isSome #inp1!Stale@.staleMemVToP);
-            Assert #execVal!Exec@.memVAddr == (getSome #inp1!Stale@.staleMemVAddr);
-            Retv
-            );
-
-          LET pcVal <- #inp1!Stale@.stalePc;
-          LET physicalPcVal <- (getSome #inp1!Stale@.staleInstVToP)!VToPRp@.pAddr;
-          LET instModeVal <- (getSome #inp1!Stale@.staleInstVToP)!VToPRp@.mode;
-          LET instExceptionVal <- (getSome #inp1!Stale@.staleInstVToP)!VToPRp@.exception;
           LET nextPcVal <- #execVal!Exec@.nextPc;
           LET execExceptionVal <- #execVal!Exec@.exception;
           LET memVAddrVal <- #execVal!Exec@.memVAddr;
-          LET memPAddrVal <- (getSome #inp1!Stale@.staleMemVToP)!VToPRp@.pAddr;
-          LET memModeVal <- (getSome #inp1!Stale@.staleMemVToP)!VToPRp@.mode;
-          LET memExceptionVal <- (getSome #inp1!Stale@.staleMemVToP)!VToPRp@.exception;
           LET dstVal <- #execVal!Exec@.data;
+
+            
+          Assert $$ (notNil stalesVal);
+          Assert $$ (isValid (sInstVToP inp1));
+          Assert $$ (isValid (sInst inp1));
+
+          If (isLdSt _ instVal)
+          then (
+            Assert $$ (isValid (sMemVAddr inp1));
+            Assert $$ (isValid (sMemVToP inp1));
+            Assert #memVAddrVal == #memVAddrVal1;
+            Retv
+            );
 
           LET cExecVal <- cExec _ pcVal physicalPcVal instModeVal instExceptionVal
               instVal nextPcVal execExceptionVal memVAddrVal memPAddrVal memModeVal
@@ -949,7 +970,10 @@ Section Processor.
               );
             Retv
             );
-          Retv }.
+
+          WriteN stales : _ <- Var _ Stales' (tl stalesVal);
+          Retv
+      }.
 
   Section Pf.
     Variable n: nat.
@@ -1092,153 +1116,119 @@ Section Processor.
       END_SKIP_PROOF_ON *) apply cheat.
     Qed.
 
-    Record VToPRpEntry := { pAddrEntry: <| PAddr |> ;
-                            modeEntry: <| Mode |> ;
-                            exceptEntry: <| optT MemException |>
-                          }.
-
-    Record Entry := { pcEntry: <| VAddr |> ;
-                      instPEntry: option VToPRpEntry ;
-                      instEntry: option <| Inst |> ;
-                      memVEntry: option <| VAddr |> ;
-                      memPEntry: option VToPRpEntry
-                    }.
-
     Definition fromInstVToPRqT (s: <| Struct InstVToPRqT |>) (v: bool) :=
       (if v then
-         Some {| pcEntry := s (InstVToPRqT !! pc);
-                 instPEntry := None;
-                 instEntry := None;
-                 memVEntry := None;
-                 memPEntry := None |}
+         Some {| sPc := s (InstVToPRqT !! pc);
+                 sInstVToP := None;
+                 sInst := None;
+                 sMemVAddr := None;
+                 sMemVToP := None |}
        else None).
                  
     Definition fromFetchRqT (s: <| Struct FetchRqT |>) (v: bool) :=
       (if v then
-         Some {| pcEntry := s (FetchRqT !! pc);
-                 instPEntry := Some {|pAddrEntry := s (FetchRqT !! physicalPc);
-                                      modeEntry := s (FetchRqT !! instMode);
-                                      exceptEntry := s (FetchRqT !! instException)
-                                    |};
-                 instEntry := None;
-                 memVEntry := None;
-                 memPEntry := None |}
+         Some {| sPc := s (FetchRqT !! pc);
+                 sInstVToP := Some {|pAddrEntry := s (FetchRqT !! physicalPc);
+                                     modeEntry := s (FetchRqT !! instMode);
+                                     exceptEntry :=
+                                       if s (FetchRqT !! instException)
+                                            ((opt MemException) !! valid)
+                                       then Some (s (FetchRqT !! instException)
+                                                    ((opt MemException) !! data))
+                                       else None
+                                   |};
+                 sInst := None;
+                 sMemVAddr := None;
+                 sMemVToP := None |}
        else None).
     
     Definition fromFetchRpT (s: <| Struct FetchRpT |>) (v: bool) :=
       (if v then
-         Some {| pcEntry := s (FetchRpT !! pc);
-                 instPEntry := Some {|pAddrEntry := s (FetchRpT !! physicalPc);
-                                      modeEntry := s (FetchRpT !! instMode);
-                                      exceptEntry := s (FetchRpT !! instException)
-                                    |};
-                 instEntry := Some (s (FetchRpT !! inst));
-                 memVEntry := None;
-                 memPEntry := None |}
+         Some {| sPc := s (FetchRpT !! pc);
+                 sInstVToP := Some {|pAddrEntry := s (FetchRpT !! physicalPc);
+                                     modeEntry := s (FetchRpT !! instMode);
+                                     exceptEntry :=
+                                       if s (FetchRpT !! instException)
+                                            ((opt MemException) !! valid)
+                                       then Some (s (FetchRpT !! instException)
+                                                    ((opt MemException) !! data))
+                                       else None
+                                   |};
+                 sInst := Some (s (FetchRpT !! inst));
+                 sMemVAddr := None;
+                 sMemVToP := None |}
        else None).
     
     Definition fromRegReadT (s: <| Struct RegReadT |>) (v: bool) :=
       (if v then
-         Some {| pcEntry := s (RegReadT !! pc);
-                 instPEntry := Some {| pAddrEntry := s (RegReadT !! physicalPc);
-                                       modeEntry := s (RegReadT !! instMode);
-                                       exceptEntry := s (RegReadT !! instException)
-                                    |};
-                 instEntry := Some (s (RegReadT !! inst));
-                 memVEntry := None;
-                 memPEntry := None |}
+         Some {| sPc := s (RegReadT !! pc);
+                 sInstVToP := Some {|pAddrEntry := s (RegReadT !! physicalPc);
+                                     modeEntry := s (RegReadT !! instMode);
+                                     exceptEntry :=
+                                       if s (RegReadT !! instException)
+                                            ((opt MemException) !! valid)
+                                       then Some (s (RegReadT !! instException)
+                                                    ((opt MemException) !! data))
+                                       else None
+                                   |};
+                 sInst := Some (s (RegReadT !! inst));
+                 sMemVAddr := None;
+                 sMemVToP := None |}
        else None).
     
     Definition fromExecT (s: <| Struct ExecT |>) (v: bool) :=
       (if v then
-         Some {| pcEntry := s (ExecT !! pc);
-                 instPEntry := Some {| pAddrEntry := s (ExecT !! physicalPc);
-                                       modeEntry := s (ExecT !! instMode);
-                                       exceptEntry := s (ExecT !! instException)
-                                    |};
-                 instEntry := Some (s (ExecT !! inst));
-                 memVEntry := Some (s (ExecT !! memVAddr));
-                 memPEntry := None |}
+         Some {| sPc := s (ExecT !! pc);
+                 sInstVToP := Some {|pAddrEntry := s (ExecT !! physicalPc);
+                                     modeEntry := s (ExecT !! instMode);
+                                     exceptEntry :=
+                                       if s (ExecT !! instException)
+                                            ((opt MemException) !! valid)
+                                       then Some (s (ExecT !! instException)
+                                                    ((opt MemException) !! data))
+                                       else None
+                                   |};
+                 sInst := Some (s (ExecT !! inst));
+                 sMemVAddr := Some (s (ExecT !! memVAddr));
+                 sMemVToP := None |}
        else None).
     
     Definition fromMemRqT (s: <| Struct MemRqT |>) (v: bool) :=
       (if v then
-         Some {| pcEntry := s (MemRqT !! pc);
-                 instPEntry := Some {| pAddrEntry := s (MemRqT !! physicalPc);
-                                       modeEntry := s (MemRqT !! instMode);
-                                       exceptEntry := s (MemRqT !! instException)
-                                    |};
-                 instEntry := Some (s (MemRqT !! inst));
-                 memVEntry := Some (s (MemRqT !! memVAddr));
-                 memPEntry := Some {| pAddrEntry := s (MemRqT !! memPAddr);
-                                      modeEntry := s (MemRqT !! memMode);
-                                      exceptEntry := s (MemRqT !! memException)
-                                    |}; |}
+         Some {| sPc := s (MemRqT !! pc);
+                 sInstVToP := Some {|pAddrEntry := s (MemRqT !! physicalPc);
+                                     modeEntry := s (MemRqT !! instMode);
+                                     exceptEntry :=
+                                       if s (MemRqT !! instException)
+                                            ((opt MemException) !! valid)
+                                       then Some (s (MemRqT !! instException)
+                                                    ((opt MemException) !! data))
+                                       else None
+                                   |};
+                 sInst := Some (s (MemRqT !! inst));
+                 sMemVAddr := Some (s (MemRqT !! memVAddr));
+                 sMemVToP := Some {|pAddrEntry := s (MemRqT !! memPAddr);
+                                    modeEntry := s (MemRqT !! memMode);
+                                    exceptEntry :=
+                                      if s (MemRqT !! memException)
+                                           ((opt MemException) !! valid)
+                                      then Some (s (MemRqT !! memException)
+                                                   ((opt MemException) !! data))
+                                      else None
+                                   |};|}
        else None).
-
-    Definition fromStale (s: <| Struct Stale |>) :=
-      {| pcEntry := s (Stale !! stalePc);
-         instPEntry :=
-           if s (Stale !! staleInstVToP) ((opt (Struct VToPRp)) !! valid)
-           then Some {| pAddrEntry := s (Stale !! staleInstVToP) ((opt (Struct VToPRp)) !! data)
-                                        (VToPRp !! pAddr);
-                        modeEntry := s (Stale !! staleInstVToP) ((opt (Struct VToPRp)) !! data)
-                                       (VToPRp !! mode);
-                        exceptEntry := s (Stale !! staleInstVToP) ((opt (Struct VToPRp)) !! data)
-                                         (VToPRp !! exception)
-                     |}
-           else None;
-         instEntry :=
-           if s (Stale !! staleInst) ((opt Inst) !! valid)
-           then Some (s (Stale !! staleInst) ((opt Inst) !! data))
-           else None;
-         memVEntry :=
-           if s (Stale !! staleMemVAddr) ((opt VAddr) !! valid)
-           then Some (s (Stale !! staleMemVAddr) ((opt VAddr) !! data))
-           else None;
-         memPEntry :=
-           if s (Stale !! staleMemVToP) ((opt (Struct VToPRp)) !! valid)
-           then Some {| pAddrEntry := s (Stale !! staleMemVToP) ((opt (Struct VToPRp)) !! data)
-                                        (VToPRp !! pAddr);
-                        modeEntry := s (Stale !! staleMemVToP) ((opt (Struct VToPRp)) !! data)
-                                       (VToPRp !! mode);
-                        exceptEntry := s (Stale !! staleMemVToP) ((opt (Struct VToPRp)) !! data)
-                                         (VToPRp !! exception)
-                     |}
-           else None;
-      |}.
-
-    Record ExecEntry := { dataEEntry: <| Data |> ;
-                          memVEEntry: <| VAddr |> ;
-                          exceptEEntry: option <| ExecException |> ;
-                          nextPcEEntry: <| VAddr |>
-                        }.
-
-    Definition execFromExecT (s: <| Struct ExecT |>) :=
-      {| dataEEntry := s (ExecT !! dst);
-         memVEEntry := s (ExecT !! memVAddr);
-         exceptEEntry := if s (ExecT !! execException) ((opt ExecException) !! valid)
-                         then Some (s (ExecT !! execException)
-                                      ((opt ExecException) !! data))
-                         else None;
-         nextPcEEntry := s (ExecT !! nextPc) |}.
+    
+    Definition execExecT (s1: <| Struct ExecT |>) (s2: <| Struct Exec |>) :=
+      s1 (ExecT !! dst) = s2 (Exec !! data) /\
+      s1 (ExecT !! memVAddr) = s2 (Exec !! memVAddr) /\
+      s1 (ExecT !! execException) = s2 (Exec !! exception) /\
+      s1 (ExecT !! nextPc) = s2 (Exec !! nextPc).
               
-    Definition execFromMemRqT (s: <| Struct MemRqT |>) :=
-      {| dataEEntry := s (MemRqT !! dst);
-         memVEEntry := s (MemRqT !! memVAddr);
-         exceptEEntry := if s (MemRqT !! execException) ((opt ExecException) !! valid)
-                         then Some (s (MemRqT !! execException)
-                                      ((opt ExecException) !! data))
-                         else None;
-         nextPcEEntry := s (MemRqT !! nextPc) |}.
-
-    Definition execFromExec (s: <| Struct Exec |>) :=
-      {| dataEEntry := s (Exec !! data);
-         memVEEntry := s (Exec !! memVAddr);
-         exceptEEntry := if s (Exec !! exception) ((opt ExecException) !! valid)
-                         then Some (s (Exec !! exception) ((opt ExecException) !! data))
-                         else None;
-         nextPcEEntry := s (Exec !! nextPc) |}.
+    Definition execMemRqT (s1: <| Struct MemRqT |>) (s2: <| Struct Exec |>) :=
+      s1 (MemRqT !! dst) = s2 (Exec !! data) /\
+      s1 (MemRqT !! memVAddr) = s2 (Exec !! memVAddr) /\
+      s1 (MemRqT !! execException) = s2 (Exec !! exception) /\
+      s1 (MemRqT !! nextPc) = s2 (Exec !! nextPc).
 
     Definition rfFromExecT (s: <| Struct ExecT |>) (e: bool) (rf: <| Vector Data RIndexSz |>) :=
       if bool_dec (s (ExecT !! wbEpoch)) e
@@ -1354,31 +1344,31 @@ Section Processor.
         execVal:
           execValid = true ->
           execData (ExecT !! wbEpoch) = wbEpochI ->
-          execFromExecT execData =
-          execFromExec (evalExpr
-                          (execFn _ (execData (ExecT !! inst))
-                                  (rfFromMemRqT memRqData memRqValid regFileS
-                                                (evalExpr (getSrc1 _ (execData (ExecT !! inst)))))
-                                  (rfFromMemRqT memRqData memRqValid regFileS
-                                                (evalExpr (getSrc2 _ (execData (ExecT !! inst)))))
-                          )%kami_expr) ;
+          execExecT execData
+                    (evalExpr
+                       (execFn _ (execData (ExecT !! inst))
+                               (rfFromMemRqT memRqData memRqValid regFileS
+                                             (evalExpr (getSrc1 _ (execData (ExecT !! inst)))))
+                               (rfFromMemRqT memRqData memRqValid regFileS
+                                             (evalExpr (getSrc2 _ (execData (ExecT !! inst)))))
+                       )%kami_expr) ;
 
         memRqVal:
           memRqValid = true ->
           memRqData (MemRqT !! wbEpoch) = wbEpochI ->
-          execFromMemRqT memRqData =
-          execFromExec (evalExpr
-                          (execFn _ (memRqData (MemRqT !! inst))
-                                  (regFileS (evalExpr (getSrc1 _ (memRqData (MemRqT !! inst)))))
-                                  (regFileS (evalExpr (getSrc2 _ (memRqData (MemRqT !! inst)))))
-                          )%kami_expr) ;
+          execMemRqT memRqData
+                     (evalExpr
+                        (execFn _ (memRqData (MemRqT !! inst))
+                                (regFileS (evalExpr (getSrc1 _ (memRqData (MemRqT !! inst)))))
+                                (regFileS (evalExpr (getSrc2 _ (memRqData (MemRqT !! inst)))))
+                        )%kami_expr) ;
 
         wbPcSFind: wbPcI === s.[wbPc] ;
         modeSFind: modeI === s.[mode] ;
         regFileSFind: regFileS === s.[regFile] ;
         cStateSFind: cStateI === s.[cState] ;
 
-        staleList: <[ list (type StaleT) ]> ;
+        staleList: <[ list (@Stale type) ]> ;
         staleListFind: staleList === s.[stales] ;
 
         listMatch:
@@ -1388,7 +1378,7 @@ Section Processor.
                              fromFetchRpT fetchRpData fetchRpValid ::
                              fromFetchRqT fetchRqData fetchRqValid ::
                              fromInstVToPRqT instVToPRqData instVToPRqValid :: nil)
-          = map fromStale staleList ;
+          = staleList ;
 
       }.
 
@@ -1412,52 +1402,64 @@ Section Processor.
     Lemma instVToPRq_inv:
       ruleMapInst combined_inv procInlUnfold procSpec instVToPRq.
     Proof.
-      (* SKIP_PROOF_ON
+      (* SKIP_PROOF_OFF *)
       initInvRight procSpec (stalePc).
-      rewrite map_app.
-      rewrite (rmNonePartition 4) in listMatch.
       rewrite (rmNonePartition 4).
-      cbv [partition fst snd] in *.
+      cbv [partition fst snd].
       simplBoolFalse.
       f_equal.
-      - procSpecificUnfold; rmNoneNilLtac; auto.
-      - reflexivity.
-      END_SKIP_PROOF_ON *) apply cheat.
+      instantiate (1 := regV).
+      reflexivity.
+      (* END_SKIP_PROOF_OFF *)
     Qed.
 
     Lemma wb_inv:
       ruleMapInst combined_inv procInlUnfold procSpec wb.
     Proof.
-      (* SKIP_PROOF_ON
+      (* SKIP_PROOF_OFF *)
       simplInv; left;
         simplInvHyp;
         simplInvGoal.
-      END_SKIP_PROOF_ON *) apply cheat.
+      (* END_SKIP_PROOF_OFF *)
     Qed.
 
-Require Import Kami.MapReifyEx.
-    
     Lemma fetchRq_inv:
       ruleMapInst combined_inv procInlUnfold procSpec fetchRq.
     Proof.
-      initInvRight procSpec (staleInstVToP). 
+      initInvRight procSpec (staleInstVToP).
       - unfold indexIn.
         cbv [evalExpr].
-        rewrite (rmNonePartition 4) in listMatch.
-        cbv [partition fst snd] in *.
-        clear - listMatch.
-        apply (f_equal (@length _)) in listMatch.
-        rewrite map_length, app_length in listMatch.
-        match type of listMatch with
-        | ?P + _ = ?Q =>
+        rewrite (rmNonePartition 4).
+        cbv [partition fst snd].
+        rewrite app_length.
+        match goal with
+        | |- context[(?P + ?Q)%nat] =>
           let cmp := fresh "cmp" in
-          assert (cmp: (P < Q)%nat) by (simpl in *; Omega.omega);
-          instantiate (1 := P)
+          assert (cmp: (P < P+Q)%nat) by (simpl in *; Omega.omega);
+            instantiate (1 := P)
         end.
         match goal with
         | |- context [if ?P then _ else _] => destruct P; auto
         end.
-      - rewrite ?evalExprRewrite.
+      - reflexivity.
+      - rewrite M.union_empty_L.
+        setoid_rewrite (rmNonePartition 4) at 2.
+        cbv [partition fst snd].
+        unfold rmNone at 3.
+        unfold fromInstVToPRqT.
+        rewrite nth_len.
+        reflexivity.
+      - apply M.Disj_empty_2.
+      - apply M.Disj_empty_2.
+      - admit.
+      - 
+        right; let X := fresh in intro X; simpl in X;
+                                   apply M.F.P.F.empty_in_iff in X.
+        assumption.
+      - constructor.
+          
+        repeat f_equal.
+        rewrite ?evalExprRewrite.
         match goal with
         | |- context[evalExpr (# (evalExpr ?P))%kami_expr] =>
           idtac
